fix lifting

deps/poulet4/lib/P4cub/Semantics/Dynamic/BigStep/Properties.v
@@ -1,21 +1,195 @@
+Require Import Coq.Arith.PeanoNat.
 From Poulet4 Require Import P4cub.Syntax.Syntax
-     P4cub.Semantics.Climate Utils.ForallMap.
+  P4cub.Semantics.Climate Utils.ForallMap
+  P4cub.Syntax.Shift.
 From Poulet4.P4cub.Semantics.Dynamic Require Import
      BigStep.Value.Syntax BigStep.Semantics BigStep.IndPrincip
      BigStep.Value.Typing.
 Import AllCubNotations Val.ValueNotations
-       Val.LValueNotations.
+  Val.LValueNotations Nat.
 
-Section Properties.  
+Ltac len_app :=
+  match goal with
+| hlen: length ?l1 = length ?l2, happ: ?l1 ++ _ = ?l2 ++ _
+  |- _ => pose proof sublist.app_eq_len_eq happ hlen as [? ?]; subst
+  end.
+
+Variant ctx_cuttoff (m : nat) : ctx -> Prop :=
+  | ctx_cuttoff_action aa :
+    ctx_cuttoff m (CAction aa)
+  | ctx_cuttoff_function :
+    ctx_cuttoff m CFunction
+  | ctx_cuttoff_applyblock ts aa ac :
+    ctx_cuttoff m (CApplyBlock ts aa ac)
+  | ctx_cuttoff_parserstate n strt sts ap :
+    n <= m ->
+    ctx_cuttoff m (CParserState n strt sts ap).
+
+Section Properties.
+  Local Hint Constructors ctx_cuttoff : core.
+
+  Lemma ctx_cuttoff_le : forall l m c,
+      m <= l ->
+      ctx_cuttoff m c ->
+      ctx_cuttoff l c.
+  Proof using.
+    intros l m c hml hc; inv hc; auto.
+    constructor. lia.
+  Qed.
+
+  Local Hint Resolve ctx_cuttoff_le : core.
   Local Hint Resolve ForallMap.Forall2_dumb : core.
   Local Hint Constructors expr_big_step : core.
-  Local Hint Constructors stmt_big_step : core.
+  Local Hint Extern 1 => len_app : core.
+
+  Lemma shift_e_eval : forall us vs ϵ e v,
+      ⟨ us ++ ϵ, e ⟩ ⇓ v ->
+      ⟨ us ++ vs ++ ϵ,
+        shift_e
+          (Shifter (length us) (length vs)) e ⟩ ⇓ v.
+  Proof using.
+    intros us vs ϵ e v h.
+    remember (us ++ ϵ) as usϵ eqn:husϵ.
+    generalize dependent ϵ.
+    generalize dependent us.
+    induction h using custom_expr_big_step_ind;
+      intros us eps huseps; subst;
+      unravel; eauto.
+    - unfold shift_var. unravel.
+      constructor. destruct_if.
+      + rewrite nth_error_app2 in * by lia.
+        rewrite <- Nat.add_sub_assoc by lia.
+        rewrite nth_error_app3.
+        assumption.
+      + rewrite nth_error_app1 in * by lia.
+        assumption.
+    - rewrite Forall2_forall_nth_error in H0.
+      destruct H0 as [Hlen HF2].
+      pose proof
+        (conj Hlen
+           (fun n e v he hv =>
+              HF2 n e v he hv us eps Logic.eq_refl))
+        as HF2'.
+      rewrite <- Forall2_forall_nth_error in HF2'.
+      clear HF2 Hlen.
+      constructor.
+      rewrite sublist.Forall2_map1.
+      assumption.
+  Qed.
+
+  Local Hint Resolve shift_e_eval : core.
+  Local Hint Constructors parser_expr_big_step : core.
+
+  Lemma shift_trans_eval : forall us ϵ p st,
+      p⟨ us ++ ϵ , p ⟩ ⇓ st -> forall vs,
+        p⟨ us ++ vs ++ ϵ , shift_transition (Shifter (length us) (length vs)) p ⟩ ⇓ st.
+  Proof using.
+    intros us eps p st h vs.
+    inv h; unravel; auto.
+  Qed.
+
+  Local Hint Resolve shift_trans_eval : core.
+
+  Fixpoint shift_lv (sh : shifter) (lv : Val.lv) : Val.lv :=
+  match lv with
+  | Val.Var x => Val.Var $ shift_var sh x
+  | Val.Slice hi lo lv => Val.Slice hi lo $ shift_lv sh lv
+  | Val.Member x lv => Val.Member x $ shift_lv sh lv
+  | Val.Index n lv => Val.Index n $ shift_lv sh lv
+  end.
+
+  Lemma shift_lv_0_add : forall lv m n,
+      shift_lv (Shifter 0 (m + n)) lv = shift_lv (Shifter 0 m) (shift_lv (Shifter 0 n) lv).
+  Proof using.
+    intro lv; induction lv; intros m n; unravel; f_equal; auto.
+    unfold shift_var; cbn. lia.
+  Qed.
+  
+  Lemma shift_lv_0 : forall lv c, shift_lv (Shifter c 0) lv = lv.
+  Proof using.
+    intros lv c; induction lv; unravel; f_equal; auto.
+    unfold shift_var. destruct_if; reflexivity.
+  Qed.
+  
+  Local Hint Constructors lexpr_big_step : core.
+
+  Lemma shift_lv_eval : forall us vs ϵ e lv,
+      l⟨ us ++ ϵ, e ⟩ ⇓ lv ->
+      l⟨ us ++ vs ++ ϵ,
+          shift_e
+            (Shifter (length us) (length vs)) e ⟩
+        ⇓ shift_lv (Shifter (length us) (length vs)) lv.
+  Proof using.
+    intros us vs eps e lv h.
+    remember (us ++ eps) as useps eqn:huseps.
+    generalize dependent eps.
+    generalize dependent us.
+    induction h; intros; subst; unravel; eauto.
+  Qed.
+
+  Local Hint Resolve shift_lv_eval : core.
+
+  Lemma shift_lv_lookup : forall lv rs us ϵ,
+      lv_lookup (rs ++ us ++ ϵ) (shift_lv (Shifter (length rs) (length us)) lv)
+      = lv_lookup (rs ++ ϵ) lv.
+  Proof using.
+    intro lv; induction lv; intros; unravel.
+    - unfold shift_var, cutoff,amt.
+      destruct_if.
+      + rewrite nth_error_app2
+          with (n := x) by assumption.
+        rewrite nth_error_app2
+          with (n := length us + x) by lia.
+        replace (length us + x - length rs)
+          with (length us + (x - length rs)) by lia.
+        rewrite nth_error_app3.
+        reflexivity.
+      + rewrite nth_error_app1 by lia.
+        rewrite nth_error_app1 by assumption.
+        reflexivity.
+    - rewrite IHlv. reflexivity.
+    - rewrite IHlv. reflexivity.
+    - rewrite IHlv. reflexivity.
+  Qed.
+
+  Local Hint Rewrite shift_lv_lookup : core.
+
+  Lemma shift_lv_update : forall lv v rs ϵ rs' ϵ',
+      length rs = length rs' ->
+      lv_update lv v (rs ++ ϵ) = rs' ++ ϵ' -> forall us,
+          lv_update (shift_lv (Shifter (length rs) (length us)) lv) v (rs ++ us ++ ϵ)
+          = rs' ++ us ++ ϵ'.
+  Proof using.
+    intro lv; induction lv;
+      intros v rs eps rs' eps' hrs hlv us;
+      unravel in *; autorewrite with core.
+    - unfold shift_var, cutoff, amt.
+      destruct_if.
+      + rewrite nth_update_app1 in * by lia.
+        replace (length us + x - length rs)
+          with (length us + (x - length rs)) by lia.
+        rewrite nth_update_app3.
+        pose proof sublist.app_eq_len_eq hlv hrs as [hrs' heps]; subst.
+        reflexivity.
+      + rewrite nth_update_app2 in * by lia.
+        assert (length (nth_update x v rs) = length rs') as hup.
+      { rewrite nth_update_length. assumption. }
+      pose proof sublist.app_eq_len_eq hlv hup as [hrs' heps]; subst.
+      reflexivity.
+    - destruct v; auto.
+      destruct (lv_lookup (rs ++ eps) lv) as [[] |]; auto.
+    - destruct (lv_lookup (rs ++ eps) lv) as [[] |]; auto.
+      destruct ls; eauto.
+    - destruct (lv_lookup (rs ++ eps) lv) as [[] |]; auto.
+      destruct ls; eauto.
+  Qed.
+
   Local Hint Resolve lv_update_length : core.
   Local Hint Rewrite lv_update_length : core.
-
+  
   Lemma lv_update_signal_length : forall olv sig ϵ,
       length (lv_update_signal olv sig ϵ) = length ϵ.
-  Proof.
+  Proof using.
     intros [] [| | | | []] ϵ; cbn; auto.
   Qed.
 
@@ -24,7 +198,7 @@ Section Properties.
   
   Lemma copy_out_from_args_length : forall vs₁ vs₂ ϵ,
       length (copy_out_from_args vs₁ vs₂ ϵ) = length ϵ.
-  Proof.
+  Proof using.
     intro vs1; induction vs1 as [| [] vs1 ih];
       intros [| [] vs2] ϵ; cbn in *;
       try rewrite ih; auto.
@@ -41,8 +215,124 @@ Section Properties.
   
   Lemma sbs_length : forall Ψ ϵ ϵ' c s sig ψ,
       ⧼ Ψ, ϵ, c, s ⧽ ⤋ ⧼ ϵ', sig, ψ ⧽ -> length ϵ = length ϵ'.
-  Proof.
+  Proof using.
     intros Ψ ϵ ϵ' c s sig ψ h;
       induction h; autorewrite with core in *; auto; lia.
   Qed.
+
+  Local Hint Constructors relop : core.
+  Local Hint Constructors stmt_big_step : core.
+  
+  Lemma shift_s_eval : forall Ψ us us' ϵ ϵ' c s sig ψ,
+      length us = length us' ->
+      ctx_cuttoff (length ϵ) c ->
+      ⧼ Ψ , us ++ ϵ , c , s ⧽ ⤋ ⧼ us' ++ ϵ' , sig , ψ ⧽ -> forall vs,
+          ⧼ Ψ , us ++ vs ++ ϵ , c ,
+            shift_s (Shifter (length us) (length vs)) s ⧽
+            ⤋ ⧼ us' ++ vs ++ ϵ' , sig , ψ ⧽.
+  Proof using.
+    intros Psi us us' eps eps' c s sig psi hus hc hs.
+    remember (us ++ eps) as useps eqn:huseps.
+    remember (us' ++ eps') as useps' eqn:huseps'.
+    generalize dependent eps'.
+    generalize dependent us'.
+    generalize dependent eps.
+    generalize dependent us.
+    induction hs; intros; unravel; subst; eauto.
+    - inv H; unravel; auto.
+    - pose proof sbs_length _ _ _ _ _ _ _ hs as hlen.
+      pose proof app_eq_app _ _ _ _ huseps as [l2 heps2].
+      pose proof app_eq_app _ _ _ _ huseps' as [l3 heps3].
+      inv hc.
+      destruct heps2 as [[hl2 heps2] | [hl2 hesp2]];
+        destruct heps3 as [[hl3 heps3] | [hl3 hesp3]]; subst.
+      + rewrite <- app_assoc in huseps,  huseps'.
+        pose proof sublist.app_eq_len_eq huseps' hus as [huseq heps]; subst.
+        rewrite app_inv_head_iff in hl3, huseps'; subst.
+        do 4 rewrite app_assoc.
+        econstructor; eauto.
+        rewrite <- app_assoc in H1.
+        do 2 rewrite <- app_assoc.
+        eauto.
+      + rewrite <- app_assoc in hus.
+        repeat rewrite app_length in *.
+        assert (hlen2 : length l2 = 0) by lia.
+        assert (hlen3 : length l3 = 0) by lia.
+        rewrite length_zero_iff_nil in hlen2.
+        rewrite length_zero_iff_nil in hlen3.
+        subst; cbn in *.
+        repeat rewrite <- app_assoc in *; cbn in *.
+        do 2 rewrite app_assoc.
+        econstructor; eauto.
+        rewrite <- app_assoc.
+        eauto.
+      + rewrite <- app_assoc in hus.
+        repeat rewrite app_length in *.
+        assert (hlen2 : length l2 = 0) by lia.
+        assert (hlen3 : length l3 = 0) by lia.
+        rewrite length_zero_iff_nil in hlen2.
+        rewrite length_zero_iff_nil in hlen3.
+        subst; cbn in *.
+        repeat rewrite <- app_assoc in *; cbn in *.
+        do 2 rewrite app_assoc.
+        econstructor; eauto.
+        rewrite <- app_assoc.
+        do 2 rewrite add_0_r.
+        eauto.
+      + repeat rewrite app_length in * |-.
+        assert (hl23 : length l2 = length l3) by lia.
+        assert (hepslen : length eps = length eps') by lia.
+        assert (hlen2 : length l2 = 0) by lia.
+        rewrite length_zero_iff_nil in hlen2.
+        subst; cbn in *.
+        symmetry in hl23.
+        rewrite length_zero_iff_nil in hl23.
+        subst; cbn in *.
+        repeat rewrite app_nil_r.
+        do 2 rewrite app_assoc.
+        econstructor; eauto.
+        rewrite <- app_assoc. auto.
+    - pose proof shift_lv_update _ _ _ _ _ _ hus huseps' vs as hvs.
+      rewrite <- hvs.
+      constructor; auto.
+    - admit.
+    - admit.
+    - admit.
+    - admit.
+    - admit.
+    - admit.
+    - destruct te as [t | e]; unravel; unfold shext,smother,RecordSet.set; cbn.
+      + apply sbs_var with (v := v) (v' := v'); auto.
+        replace (v :: us ++ vs ++ eps)
+          with ((v :: us) ++ vs ++ eps) by reflexivity.
+        replace (v' :: us' ++ vs ++ eps')
+          with ((v' :: us') ++ vs ++ eps') by reflexivity.
+        replace (S (length us)) with (length (v :: us)) by reflexivity.
+        apply IHhs; cbn; auto.
+      + apply sbs_var with (v := v) (v' := v'); auto.
+        replace (v :: us ++ vs ++ eps)
+          with ((v :: us) ++ vs ++ eps) by reflexivity.
+        replace (v' :: us' ++ vs ++ eps')
+          with ((v' :: us') ++ vs ++ eps') by reflexivity.
+        replace (S (length us)) with (length (v :: us)) by reflexivity.
+        apply IHhs; cbn; auto.
+    - assert (hϵ' : length (us ++ eps) = length ϵ') by
+        eauto using sbs_length.
+      rewrite app_length in hϵ'.
+      eapply sbs_seq_cont with (ϵ' := firstn (length us) ϵ' ++ vs ++ skipn (length us) ϵ'); eauto.
+      + eapply IHhs1; eauto.
+        * rewrite firstn_length. lia.
+        * rewrite firstn_skipn. reflexivity.
+      + replace (length us) with
+          (length (firstn (length us) ϵ')) at 3
+          by (rewrite firstn_length; lia).
+        eapply IHhs2; eauto.
+        * rewrite skipn_length, <- hϵ'.
+          replace (length us + length eps - length us) with (length eps) by lia.
+          assumption.
+        * rewrite firstn_skipn. reflexivity.
+        * rewrite firstn_length; lia.
+    - econstructor; eauto.
+      destruct b; auto.
+  Admitted.
 End Properties.
