deps/poulet4/lib/P4cub/Transformations/Lifting/Lift.v
@@ -14,252 +14,6 @@ Import RecordSetNotations.
 Open Scope nat_scope.
 Open Scope string_scope.
 Open Scope list_scope.
-
-Ltac len_app :=
-  match goal with
-| hlen: length ?l1 = length ?l2, happ: ?l1 ++ _ = ?l2 ++ _
-  |- _ => pose proof sublist.app_eq_len_eq happ hlen as [? ?]; subst
-  end.
-
-Local Hint Extern 1 => len_app : core.
-
-Lemma shift_e_0 : forall e c, shift_e (Shifter c 0) e = e.
-Proof.
-  intros e c.
-  induction e using custom_e_ind; unravel;
-    f_equal; auto.
-  - unfold shift_var.
-    destruct_if; reflexivity.
-  - apply map_ext_Forall in H.
-    rewrite H, map_id; reflexivity.
-Qed.
-
-Local Hint Rewrite shift_e_0 : core.
-
-Lemma shift_e_0_map : forall es c,
-    map (shift_e (Shifter c 0)) es = es.
-Proof.
-  intros es c;
-    induction es as [| e es ih]; unravel;
-    autorewrite with core; f_equal; auto.
-Qed.
-
-Local Hint Rewrite shift_e_0_map : core.
-
-Lemma shift_arg_0 : forall arg c, shift_arg (Shifter c 0) arg = arg.
-Proof.
-  intros [] c; unravel;
-    autorewrite with core; reflexivity.
-Qed.
-
-Local Hint Rewrite shift_arg_0 : core.
-
-Lemma shift_arg_0_map : forall args c,
-    map (shift_arg (Shifter c 0)) args = args.
-Proof.
-  intros args c;
-    induction args as [| arg args ih];
-    unravel; autorewrite with core;
-    f_equal; auto.
-Qed.
-
-Local Hint Rewrite shift_arg_0_map : core.
-
-Lemma shift_trans_0 : forall p c, shift_transition (Shifter c 0) p = p.
-Proof.
-  intros [] c; unravel;
-    autorewrite with core; reflexivity.
-Qed.
-
-Local Hint Rewrite shift_trans_0 : core.
-
-Lemma shift_s_0 : forall s c, shift_s (Shifter c 0) s = s.
-Proof.
-  intro s;
-    induction s;
-    intro c; unravel;
-    autorewrite with core;
-    unfold sext, smother, RecordSet.set; unravel;
-    f_equal; auto.
-  - destruct e; unravel;
-      autorewrite with core; reflexivity.
-  - destruct expr; unravel;
-      autorewrite with core; reflexivity.
-Qed.
-
-Local Hint Constructors expr_big_step : core.
-
-Lemma shift_e_eval : forall us vs ϵ e v,
-    ⟨ us ++ ϵ, e ⟩ ⇓ v ->
-    ⟨ us ++ vs ++ ϵ,
-      shift_e
-        (Shifter (length us) (length vs)) e ⟩ ⇓ v.
-Proof.
-  intros us vs ϵ e v h.
-  remember (us ++ ϵ) as usϵ eqn:husϵ.
-  generalize dependent ϵ.
-  generalize dependent us.
-  induction h using custom_expr_big_step_ind;
-    intros us eps huseps; subst;
-    unravel; eauto.
-  - unfold shift_var. unravel.
-    constructor. destruct_if.
-    + rewrite nth_error_app2 in * by lia.
-      rewrite <- Nat.add_sub_assoc by lia.
-      rewrite nth_error_app3.
-      assumption.
-    + rewrite nth_error_app1 in * by lia.
-      assumption.
-  - rewrite Forall2_forall_nth_error in H0.
-    destruct H0 as [Hlen HF2].
-    pose proof
-      (conj Hlen
-         (fun n e v he hv =>
-            HF2 n e v he hv us eps Logic.eq_refl))
-      as HF2'.
-    rewrite <- Forall2_forall_nth_error in HF2'.
-    clear HF2 Hlen.
-    constructor.
-    rewrite sublist.Forall2_map1.
-    assumption.
-Qed.
-
-Local Hint Resolve shift_e_eval : core.
-Local Hint Constructors parser_expr_big_step : core.
-
-Lemma shift_trans_eval : forall us ϵ p st,
-    p⟨ us ++ ϵ , p ⟩ ⇓ st -> forall vs,
-      p⟨ us ++ vs ++ ϵ , shift_transition (Shifter (length us) (length vs)) p ⟩ ⇓ st.
-Proof.
-  intros us eps p st h vs.
-  inv h; unravel; auto.
-Qed.
-
-Local Hint Resolve shift_trans_eval : core.
-
-Fixpoint shift_lv (sh : shifter) (lv : Val.lv) : Val.lv :=
-  match lv with
-  | Val.Var x => Val.Var $ shift_var sh x
-  | Val.Slice hi lo lv => Val.Slice hi lo $ shift_lv sh lv
-  | Val.Member x lv => Val.Member x $ shift_lv sh lv
-  | Val.Index n lv => Val.Index n $ shift_lv sh lv
-  end.
-
-Lemma shift_lv_0_add : forall lv m n,
-    shift_lv (Shifter 0 (m + n)) lv = shift_lv (Shifter 0 m) (shift_lv (Shifter 0 n) lv).
-Proof.
-  intro lv; induction lv; intros m n; unravel; f_equal; auto.
-  unfold shift_var; cbn. lia.
-Qed.
-
-Lemma shift_lv_0 : forall lv c, shift_lv (Shifter c 0) lv = lv.
-Proof.
-  intros lv c; induction lv; unravel; f_equal; auto.
-  unfold shift_var. destruct_if; reflexivity.
-Qed.
-
-Local Hint Constructors lexpr_big_step : core.
-
-Lemma shift_lv_eval : forall us vs ϵ e lv,
-    l⟨ us ++ ϵ, e ⟩ ⇓ lv ->
-    l⟨ us ++ vs ++ ϵ,
-        shift_e
-          (Shifter (length us) (length vs)) e ⟩
-      ⇓ shift_lv (Shifter (length us) (length vs)) lv.
-Proof.
-  intros us vs eps e lv h.
-  remember (us ++ eps) as useps eqn:huseps.
-  generalize dependent eps.
-  generalize dependent us.
-  induction h; intros; subst; unravel; eauto.
-Qed.
-
-Local Hint Resolve shift_lv_eval : core.
-
-Lemma nth_update_app1 : forall {A : Set} n (a : A) l1 l2,
-    length l1 <= n ->
-    nth_update n a (l1 ++ l2) = l1 ++ nth_update (n - length l1) a l2.
-Proof.
-  intros A n a;
-    induction n as [| n ih];
-    intros [| a1 l1] l2 h; cbn in *;
-    lia || (f_equal; auto).
-  apply ih. lia.
-Qed.
-
-Lemma nth_update_app2 : forall {A : Set} n (a : A) l1 l2,
-    n < length l1 ->
-    nth_update n a (l1 ++ l2) = nth_update n a l1 ++ l2.
-Proof.
-  intros A n a;
-    induction n as [| n ih];
-    intros [| a1 l1] l2 h; cbn in *;
-    lia || (f_equal; auto).
-  apply ih. lia.
-Qed.
-
-Lemma nth_update_app3 : forall {A : Set} n (a : A) l1 l2,
-    nth_update (length l1 + n) a (l1 ++ l2) = l1 ++ nth_update n a l2.
-Proof.
-  intros.
-  rewrite nth_update_app1 by lia.
-  f_equal. f_equal. lia.
-Qed.
-
-Lemma shift_lv_lookup : forall lv rs us ϵ,
-    lv_lookup (rs ++ us ++ ϵ) (shift_lv (Shifter (length rs) (length us)) lv)
-    = lv_lookup (rs ++ ϵ) lv.
-Proof.
-  intro lv; induction lv; intros; unravel.
-  - unfold shift_var, cutoff,amt.
-    destruct_if.
-    + rewrite nth_error_app2
-        with (n := x) by assumption.
-      rewrite nth_error_app2
-        with (n := length us + x) by lia.
-      replace (length us + x - length rs)
-        with (length us + (x - length rs)) by lia.
-      rewrite nth_error_app3.
-      reflexivity.
-    + rewrite nth_error_app1 by lia.
-      rewrite nth_error_app1 by assumption.
-      reflexivity.
-  - rewrite IHlv. reflexivity.
-  - rewrite IHlv. reflexivity.
-  - rewrite IHlv. reflexivity.
-Qed.
-
-Local Hint Rewrite shift_lv_lookup : core.
-
-Lemma shift_lv_update : forall lv v rs ϵ rs' ϵ',
-    length rs = length rs' ->
-    lv_update lv v (rs ++ ϵ) = rs' ++ ϵ' -> forall us,
-      lv_update (shift_lv (Shifter (length rs) (length us)) lv) v (rs ++ us ++ ϵ)
-      = rs' ++ us ++ ϵ'.
-Proof.
-  intro lv; induction lv;
-    intros v rs eps rs' eps' hrs hlv us;
-    unravel in *; autorewrite with core.
-  - unfold shift_var, cutoff, amt.
-    destruct_if.
-    + rewrite nth_update_app1 in * by lia.
-      replace (length us + x - length rs)
-        with (length us + (x - length rs)) by lia.
-      rewrite nth_update_app3.
-      pose proof sublist.app_eq_len_eq hlv hrs as [hrs' heps]; subst.
-      reflexivity.
-    + rewrite nth_update_app2 in * by lia.
-      assert (length (nth_update x v rs) = length rs') as hup.
-      { rewrite nth_update_length. assumption. }
-      pose proof sublist.app_eq_len_eq hlv hup as [hrs' heps]; subst.
-      reflexivity.
-  - destruct v; auto.
-    destruct (lv_lookup (rs ++ eps) lv) as [[] |]; auto.
-  - destruct (lv_lookup (rs ++ eps) lv) as [[] |]; auto.
-    destruct ls; eauto.
-  - destruct (lv_lookup (rs ++ eps) lv) as [[] |]; auto.
-    destruct ls; eauto.
-Qed.
     
 Inductive eval_decl_list
   (ϵ : list Val.v)
@@ -297,12 +51,7 @@ Proof.
 Qed.
 
 Local Hint Resolve eval_decl_list_length : core.
-
-Fixpoint shift_elist (sh : shifter) (es : list Expr.e) : list Expr.e :=
-  match es with
-  | [] => []
-  | e :: es => shift_e (smother sh (length es)) e :: shift_elist sh es
-  end.
+Local Hint Resolve shift_e_eval : core.
 
 Lemma eval_decl_list_app : forall ϵ es1 es2 vs1 vs2,
     eval_decl_list ϵ es1 vs1 ->
@@ -326,21 +75,72 @@ Local Hint Resolve eval_decl_list_app : core.
 Local Open Scope expr_scope.
 Local Open Scope stmt_scope.
 
+Fixpoint shift_pairs (ess : list (Expr.e * list Expr.e)) : list (Expr.e * list Expr.e) :=
+  match ess with
+  | [] => []
+  | (e,es) :: ess
+    => let n := list_sum $ map (@length _) $ map snd ess in
+      (shift_e (Shifter (length es) n) e,
+        shift_elist (Shifter 0 n) es) ::
+        map (fun '(e,es') => (shift_e (Shifter 0 $ length es) e, es')) (shift_pairs ess)
+  end.
+
+Lemma shift_one_pair : forall e es,
+    shift_pairs [(e,es)] = [(e,es)].
+Proof.
+  intros; cbn; rewrite shift_e_0 , shift_elist_0. reflexivity.
+Qed.
+
+Lemma shift_two_pairs : forall e1 e2 es1 es2,
+    shift_pairs [(e2,es2);(e1,es1)]
+    = [(shift_e (Shifter (length es2) (length es1)) e2,
+         shift_elist (Shifter 0 (length es1)) es2);
+       (shift_e (Shifter 0 (length es2)) e1, es1)].
+Proof.
+  intros; unravel.
+  rewrite add_0_r, shift_elist_0, shift_e_0.
+  reflexivity.
+Qed.
+
+Lemma shift_three_pairs : forall e1 e2 e3 es1 es2 es3,
+    shift_pairs [(e3,es3);(e2,es2);(e1,es1)]
+    = [(shift_e (Shifter (length es3) (length es2 + length es1)) e3,
+            shift_elist (Shifter 0 (length es2 + length es1)) es3);
+       (shift_e (Shifter 0 (length es3)) (shift_e (Shifter (length es2) (length es1)) e2),
+         shift_elist (Shifter 0 (length es1)) es2);
+       (shift_e (Shifter 0 (length es3 + length es2)) e1, es1)].
+Proof.
+  intros; unravel.
+  rewrite add_0_r, shift_elist_0, shift_e_0, shift_e_add.
+  reflexivity.
+Qed.
+       
 Inductive Lift_e
   : Expr.e -> Expr.e -> list Expr.e -> Prop :=
-| Lift_e_bool (b : bool) :
+| Lift_bool (b : bool) :
   Lift_e b b []
-| Lift_e_bit w n :
-  Lift_e (w `W n) (Expr.Var (Expr.TBit w) "" 0) [w `W n]
-| Lift_e_var t og x :
+| Lift_var t og x :
   Lift_e (Expr.Var t og x) (Expr.Var t og x) []
-| Lift_e_member t x e e' es :
+| Lift_bit w n :
+  Lift_e (w `W n) (Expr.Var (Expr.TBit w) "" 0) [w `W n]
+| Lift_int w z :
+  Lift_e (w `S z) (Expr.Var (Expr.TInt w) "" 0) [w `S z]
+| Lift_member t x e e' es :
   Lift_e e e' es ->
   Lift_e (Expr.Member t x e) (Expr.Member t x e') es
-| Lift_e_uop t o e e' es :
+| Lift_uop t o e e' es :
   Lift_e e e' es ->
   Lift_e (Expr.Uop t o e) (Expr.Var t "" 0) (Expr.Uop t o e' :: es)
-| Lift_e_index t e1 e2 e1' e2' es1 es2 :
+| Lift_slice hi lo e e' es :
+  Lift_e e e' es ->
+  Lift_e
+    (Expr.Slice hi lo e)
+    (Expr.Var (Expr.TBit (Npos hi - Npos lo + 1)%N) "" 0)
+    (Expr.Slice hi lo e' :: es)
+| Lift_cast t e e' es :
+  Lift_e e e' es ->
+  Lift_e (Expr.Cast t e) (Expr.Var t "" 0) (Expr.Cast t e' :: es)
+| Lift_index t e1 e2 e1' e2' es1 es2 :
   Lift_e e1 e1' es1 ->
   Lift_e e2 e2' es2 ->
   Lift_e
@@ -350,7 +150,7 @@ Inductive Lift_e
        (shift_e (Shifter 0 (length es2)) e1')
        (shift_e (Shifter (length es2) (length es1)) e2'))
     (shift_elist (Shifter 0 (length es1)) es2 ++ es1)
-| Lift_e_bop t o e1 e2 e1' e2' es1 es2 :
+| Lift_bop t o e1 e2 e1' e2' es1 es2 :
   Lift_e e1 e1' es1 ->
   Lift_e e2 e2' es2 ->
   Lift_e
@@ -360,7 +160,13 @@ Inductive Lift_e
        t o
        (shift_e (Shifter 0 (length es2)) e1')
        (shift_e (Shifter (length es2) (length es1)) e2')
-       :: shift_elist (Shifter 0 (length es1)) es2 ++ es1).
+       :: shift_elist (Shifter 0 (length es1)) es2 ++ es1)
+| Lift_lists ls es es' ess :
+  Forall3 Lift_e es es' ess ->
+  Lift_e
+    (Expr.Lists ls es)
+    (Expr.Var (t_of_lists ls es) "" 0)
+    (Expr.Lists ls es' :: concat ess).
 
 Lemma Lift_e_good : forall ϵ e v,
     ⟨ ϵ, e ⟩ ⇓ v -> forall e' es,
@@ -421,14 +227,14 @@ Fixpoint Unwind (es : list Expr.e) (s : Stmt.s) : Stmt.s :=
   end.
 
 Inductive Lift_s : Stmt.s -> Stmt.s -> Prop :=
-| Lift_s_skip :
+| Lift_skip :
   Lift_s Stmt.Skip Stmt.Skip
-| Lift_s_return_some e e' es :
+| Lift_return_some e e' es :
   Lift_e e e' es ->
   Lift_s
     (Stmt.Return (Some e))
     (Unwind es (Stmt.Return (Some e')))
-| Lift_s_asgn e1 e2 e1' e2' es1 es2 :
+| Lift_asgn e1 e2 e1' e2' es1 es2 :
   Lift_e e1 e1' es1 ->
   Lift_e e2 e2' es2 ->
   Lift_s
@@ -437,11 +243,11 @@ Inductive Lift_s : Stmt.s -> Stmt.s -> Prop :=
        (shift_elist (Shifter 0 (length es1)) es2 ++ es1)
        (shift_e (Shifter 0 (length es2)) e1'
           `:= shift_e (Shifter (length es2) (length es1)) e2'))
-| Lift_s_seq s1 s2 s1' s2' :
+| Lift_seq s1 s2 s1' s2' :
   Lift_s s1 s1' ->
   Lift_s s2 s2' ->
   Lift_s (s1 `; s2) (s1' `; s2')
-| Lift_s_if e e' s1 s2 s1' s2' es :
+| Lift_if e e' s1 s2 s1' s2' es :
   Lift_e e e' es ->
   Lift_s s1 s1' ->
   Lift_s s2 s2' ->
@@ -452,10 +258,10 @@ Inductive Lift_s : Stmt.s -> Stmt.s -> Prop :=
        (If e'
           Then shift_s (Shifter 0 (length es)) s1'
           Else shift_s (Shifter 0 (length es)) s2'))
-| Lift_s_var_typ og t s s' :
+| Lift_var_typ og t s s' :
   Lift_s s s' ->
   Lift_s (Stmt.Var og (inl t) s) (Stmt.Var og (inl t) s')
-| Lift_s_var_exp og e e' s s' es :
+| Lift_var_exp og e e' s s' es :
   Lift_e e e' es ->
   Lift_s s s' ->
   Lift_s
@@ -463,30 +269,6 @@ Inductive Lift_s : Stmt.s -> Stmt.s -> Prop :=
     (Unwind
        es
        (Stmt.Var og (inr e') (shift_s (Shifter 1 (length es)) s'))).
-
-Variant ctx_cuttoff (m : nat) : ctx -> Prop :=
-  | ctx_cuttoff_action aa :
-    ctx_cuttoff m (CAction aa)
-  | ctx_cuttoff_function :
-    ctx_cuttoff m CFunction
-  | ctx_cuttoff_applyblock ts aa ac :
-    ctx_cuttoff m (CApplyBlock ts aa ac)
-  | ctx_cuttoff_parserstate n strt sts ap :
-    n <= m ->
-    ctx_cuttoff m (CParserState n strt sts ap).
-
-Local Hint Constructors ctx_cuttoff : core.
-
-Lemma ctx_cuttoff_le : forall l m c,
-    m <= l ->
-    ctx_cuttoff m c ->
-    ctx_cuttoff l c.
-Proof.
-  intros l m c hml hc; inv hc; auto.
-  constructor. lia.
-Qed.
-
-Local Hint Resolve ctx_cuttoff_le : core.
 
 Section StatementLifting.
   Context `{ext_sem : Extern_Sem}.
@@ -511,123 +293,9 @@ Section StatementLifting.
   Qed.
 
   Local Hint Resolve eval_decl_list_Unwind : core.
-  
-  Lemma shift_s_eval : forall Ψ us us' ϵ ϵ' c s sig ψ,
-      length us = length us' ->
-      ctx_cuttoff (length ϵ) c ->
-      ⧼ Ψ , us ++ ϵ , c , s ⧽ ⤋ ⧼ us' ++ ϵ' , sig , ψ ⧽ -> forall vs,
-          ⧼ Ψ , us ++ vs ++ ϵ , c ,
-            shift_s (Shifter (length us) (length vs)) s ⧽
-            ⤋ ⧼ us' ++ vs ++ ϵ' , sig , ψ ⧽.
-  Proof using.
-    intros Psi us us' eps eps' c s sig psi hus hc hs.
-    remember (us ++ eps) as useps eqn:huseps.
-    remember (us' ++ eps') as useps' eqn:huseps'.
-    generalize dependent eps'.
-    generalize dependent us'.
-    generalize dependent eps.
-    generalize dependent us.
-    induction hs; intros; unravel; subst; eauto.
-    - inv H; unravel; auto.
-    - pose proof sbs_length _ _ _ _ _ _ _ hs as hlen.
-      pose proof app_eq_app _ _ _ _ huseps as [l2 heps2].
-      pose proof app_eq_app _ _ _ _ huseps' as [l3 heps3].
-      inv hc.
-      destruct heps2 as [[hl2 heps2] | [hl2 hesp2]];
-        destruct heps3 as [[hl3 heps3] | [hl3 hesp3]]; subst.
-      + rewrite <- app_assoc in huseps,  huseps'.
-        pose proof sublist.app_eq_len_eq huseps' hus as [huseq heps]; subst.
-        rewrite app_inv_head_iff in hl3, huseps'; subst.
-        do 4 rewrite app_assoc.
-        econstructor; eauto.
-        rewrite <- app_assoc in H1.
-        do 2 rewrite <- app_assoc.
-        eauto.
-      + rewrite <- app_assoc in hus.
-        repeat rewrite app_length in *.
-        assert (hlen2 : length l2 = 0) by lia.
-        assert (hlen3 : length l3 = 0) by lia.
-        rewrite length_zero_iff_nil in hlen2.
-        rewrite length_zero_iff_nil in hlen3.
-        subst; cbn in *.
-        repeat rewrite <- app_assoc in *; cbn in *.
-        do 2 rewrite app_assoc.
-        econstructor; eauto.
-        rewrite <- app_assoc.
-        eauto.
-      + rewrite <- app_assoc in hus.
-        repeat rewrite app_length in *.
-        assert (hlen2 : length l2 = 0) by lia.
-        assert (hlen3 : length l3 = 0) by lia.
-        rewrite length_zero_iff_nil in hlen2.
-        rewrite length_zero_iff_nil in hlen3.
-        subst; cbn in *.
-        repeat rewrite <- app_assoc in *; cbn in *.
-        do 2 rewrite app_assoc.
-        econstructor; eauto.
-        rewrite <- app_assoc.
-        do 2 rewrite add_0_r.
-        eauto.
-      + repeat rewrite app_length in * |-.
-        assert (hl23 : length l2 = length l3) by lia.
-        assert (hepslen : length eps = length eps') by lia.
-        assert (hlen2 : length l2 = 0) by lia.
-        rewrite length_zero_iff_nil in hlen2.
-        subst; cbn in *.
-        symmetry in hl23.
-        rewrite length_zero_iff_nil in hl23.
-        subst; cbn in *.
-        repeat rewrite app_nil_r.
-        do 2 rewrite app_assoc.
-        econstructor; eauto.
-        rewrite <- app_assoc. auto.
-    - pose proof shift_lv_update _ _ _ _ _ _ hus huseps' vs as hvs.
-      rewrite <- hvs.
-      constructor; auto.
-    - admit.
-    - admit.
-    - admit.
-    - admit.
-    - admit.
-    - admit.
-    - destruct te as [t | e]; unravel; unfold sext,smother,RecordSet.set; cbn.
-      + apply sbs_var with (v := v) (v' := v'); auto.
-        replace (v :: us ++ vs ++ eps)
-          with ((v :: us) ++ vs ++ eps) by reflexivity.
-        replace (v' :: us' ++ vs ++ eps')
-          with ((v' :: us') ++ vs ++ eps') by reflexivity.
-        replace (S (length us)) with (length (v :: us)) by reflexivity.
-        apply IHhs; cbn; auto.
-      + apply sbs_var with (v := v) (v' := v'); auto.
-        replace (v :: us ++ vs ++ eps)
-          with ((v :: us) ++ vs ++ eps) by reflexivity.
-        replace (v' :: us' ++ vs ++ eps')
-          with ((v' :: us') ++ vs ++ eps') by reflexivity.
-        replace (S (length us)) with (length (v :: us)) by reflexivity.
-        apply IHhs; cbn; auto.
-    - assert (hϵ' : length (us ++ eps) = length ϵ') by
-        eauto using sbs_length.
-      rewrite app_length in hϵ'.
-      eapply sbs_seq_cont with (ϵ' := firstn (length us) ϵ' ++ vs ++ skipn (length us) ϵ'); eauto.
-      + eapply IHhs1; eauto.
-        * rewrite firstn_length. lia.
-        * rewrite firstn_skipn. reflexivity.
-      + replace (length us) with
-          (length (firstn (length us) ϵ')) at 3
-          by (rewrite firstn_length; lia).
-        eapply IHhs2; eauto.
-        * rewrite skipn_length, <- hϵ'.
-          replace (length us + length eps - length us) with (length eps) by lia.
-          assumption.
-        * rewrite firstn_skipn. reflexivity.
-        * rewrite firstn_length; lia.
-    - econstructor; eauto.
-      destruct b; auto.
-  Admitted.
-
   Local Hint Resolve shift_s_eval : core.
   
-  Lemma Lift_E_good : forall Ψ ϵ ϵ' c s sig ψ,
+  Lemma Lift_s_good : forall Ψ ϵ ϵ' c s sig ψ,
       ctx_cuttoff (length ϵ) c ->
       ⧼ Ψ, ϵ, c, s ⧽ ⤋ ⧼ ϵ', sig, ψ ⧽ -> forall s',
           Lift_s s s' ->
